src/solswitch.c
@@ -1,5 +1,12 @@
 #include <stdint.h>
 #include <stdlib.h>
+#include <stdbool.h>
+
+#define INVALID_MSG_SIZE 0
+#define UNIQUE_MSG_SIZE 8
+#define UNIQUE_MSG_A 7
+#define UNIQUE_MSG_B 12
+#define SOLENOID_OFF 0
 
 typedef struct [[rc::refined_by("msg: nat")]] ComHandler_t{
 	// uint8_t rxMsg_buf[UNIQUE_MSG_SIZE];
@@ -10,15 +17,33 @@ typedef struct [[rc::refined_by("msg: nat")]] ComHandler_t{
 
 } ComHandler_t;
 
+typedef struct 
+[[rc::refined_by("unique_voltage: nat")]]
+// [[rc::refined_by("incoming_voltage: nat")]]
+// [[rc::refined_by("msp_activation_voltage: nat")]]
+// [[rc::refined_by("solenoid_actiavation_volatage: nat")]]
+VoltageHandler_t{
+    [[rc::field("unique_voltage @ int<u8>")]]
+	uint8_t uniqueSafetyVoltage;
+    // Aren't used for now
+    // [[rc::field("incoming_voltage @ int<u8>")]]
+	// uint8_t mainIncomingVoltage;
+    // [[rc::field("msp_activation_voltage @ int<u8>")]]
+	// uint8_t mspActivationVoltage;
+    // [[rc::field("solenoid_actiavation_volatage @ int<u8>")]]
+	// uint8_t solenoidActivationVoltage;
+}VoltageHandler_t;
+
 typedef  struct
-[[rc::refined_by("state: nat", "msg: nat")]]
+[[rc::refined_by("state: nat", "msg: nat", "voltage : nat")]]
 SolenoidSwitchingParams_t{
     [[rc::field("state @ int<size_t>")]]
     size_t state;
     [[rc::field("msg @ ComHandler_t")]]
     ComHandler_t handler;
+    [[rc::field("voltage @ VoltageHandler_t")]]
+    VoltageHandler_t voltage; 
 } SolenoidSwitchingParams_t;
-
 
 [[rc::parameters("msg: nat", "p: loc")]]
 [[rc::args("p @ &own<{msg} @ ComHandler_t>")]]
@@ -28,31 +53,27 @@ SolenoidSwitchingParams_t{
 [[rc::ensures("own p : {new_msg} @ ComHandler_t")]]
  uint8_t SCH_recieveFullMsg(ComHandler_t* handler) { return 2; /* need to return something for proof to work */ }
 
-[[rc::parameters("state: nat", "msg: nat", "p: loc")]]
-[[rc::args("p @ &own<{state, msg} @ SolenoidSwitchingParams_t>")]]
+[[rc::parameters("state: nat", "msg: nat", "p: loc", "voltage : nat")]]
+[[rc::args("p @ &own<{state, msg, voltage} @ SolenoidSwitchingParams_t>")]]
 [[rc::exists("new_state : nat")]]
-[[rc::ensures("own p : { new_state ,msg} @ SolenoidSwitchingParams_t")]]
+[[rc::ensures("own p : {new_state ,msg, voltage} @ SolenoidSwitchingParams_t")]]
 [[rc::ensures("{new_state = (if Nat.eqb state 0%nat then 1%nat else state)}")]]
 [[rc::tactics("all: try destruct state. try lia. try auto.")]]
 void SML_switchTheSolenoid( SolenoidSwitchingParams_t* ssp){
 
-	if ( 0 == ssp->state ){
+	if ( SOLENOID_OFF == ssp->state ){
 		//OUT_switchSolenoid();
 		ssp->state  = 1;
 	}
 }
 
 
-#define INVALID_MSG_SIZE 0
-#define UNIQUE_MSG_SIZE 8
-#define UNIQUE_MSG_A 7
-#define UNIQUE_MSG_B 12
 
-[[rc::parameters("state: nat", "msg: nat", "len: nat", "p: loc")]]
-[[rc::args("p @ &own<{state, msg} @ SolenoidSwitchingParams_t>", "len @ int<u8>")]]
+[[rc::parameters("state: nat", "msg: nat", "len: nat", "p: loc", "voltage : nat")]]
+[[rc::args("p @ &own<{state, msg, voltage} @ SolenoidSwitchingParams_t>", "len @ int<u8>")]]
 [[rc::exists("new_msg : nat")]]
 [[rc::exists("new_state : nat")]]
-[[rc::ensures("own p : { new_state ,new_msg} @ SolenoidSwitchingParams_t")]]
+[[rc::ensures("own p : { new_state ,new_msg, voltage} @ SolenoidSwitchingParams_t")]]
 [[rc::ensures("{((new_msg = 7%nat ∨ new_msg = 12%nat) ∧ (len = 8%nat) ∧ (state = 0%nat) -> (new_state = 1%nat)) ∨ (new_state = state)}")]]
 void SML_trySwitch(SolenoidSwitchingParams_t* ssp, uint8_t length)
 {
@@ -65,17 +86,77 @@ void SML_trySwitch(SolenoidSwitchingParams_t* ssp, uint8_t length)
     }
 }
 
-[[rc::parameters("state: nat", "msg: nat", "p: loc")]]
-[[rc::args("p @ &own<{state, msg} @ SolenoidSwitchingParams_t>")]]
+[[rc::parameters("state: nat", "msg: nat", "p: loc", "voltage : nat")]]
+[[rc::args("p @ &own<{state, msg, voltage} @ SolenoidSwitchingParams_t>")]]
 [[rc::exists("new_msg : nat")]]
 [[rc::exists("new_state : nat")]]
-[[rc::ensures("own p : { new_state ,new_msg} @ SolenoidSwitchingParams_t")]]
+[[rc::ensures("own p : {new_state ,new_msg, voltage} @ SolenoidSwitchingParams_t")]]
 //todo - how to write a spec here to descrive the desried solenoid state? how to handle rxMsgSize?
 //as i understand you cant really include SCH_recieveFullMsg return value in your spec (unless you can refine it, by using return). 
 void SML_handleReceivedMsgs(SolenoidSwitchingParams_t* ssp)
 {
     uint8_t rxMsgSize = SCH_recieveFullMsg(&ssp->handler);
     SML_trySwitch(ssp, rxMsgSize);
+}
+[[rc::parameters("time: nat")]]
+[[rc::returns("time @ int<u16>")]]
+uint16_t Timer_getCurTime();
+
+[[rc::parameters("global_time: nat")]]
+[[rc::global("global_time @ int<u16>")]]
+uint16_t curTime; // Not a global in real code. But otherwise it is a problem to reason about the output of getCurTime.
+
+#define MAX_TIME_VAL 0xFFFF
+[[rc::parameters("last_time: nat", "current_time: nat")]]
+[[rc::args("last_time @ int<u16>", "current_time @ int<u16>")]]
+[[rc::requires("{current_time ≤ last_time -> 65535 - last_time + current_time ≤ 10}")]]
+[[rc::requires("{current_time > last_time -> current_time - last_time ≤ 10}")]]
+[[rc::exists("t : nat")]]
+[[ensures("{ t = (current_time ≤ last_time ) ? (current_time - last_time) : (65535 - last_time + current_time)}")]]
+[[rc::returns("t @ int<u8>")]]
+uint8_t getSafetyVoltageHoldTime(uint16_t  startTime, uint16_t  curTime){
+    // these lines will execute untill the difference (safetyVoltageHoldTime) will be greater than 10 . 
+    // so it's leagal to store safetyVoltageHoldTime in one byte.
+    uint8_t safetyVoltageHoldTime;
+  
+    // handle edge case where timeCounter is around the max value
+    // after timeCounter is equal to MAX_TIME_VAL-1 it become equal to zero
+    if( curTime < startTime ){
+        safetyVoltageHoldTime= (MAX_TIME_VAL-startTime) + curTime;
+     }else{
+        // this lines will be execute untill the difference (safetyVoltageHoldTime) will be greater than 10 . 
+        // so the cast to uint8_t is leagal.
+        safetyVoltageHoldTime = (uint8_t) (curTime - startTime);
+     }
+    return safetyVoltageHoldTime;
+}
+
+
+#define SAFETY_VOLTAGE_TRESHOLD 217
+#define SAFETY_VOLTAGE_REQUIRED_HOLD_TIME 11
+[[rc::parameters("state: nat", "msg: nat", "conversionEnded: bool", "voltage : nat", "p: loc", "global_time : nat")]]
+[[rc::args("p @ &own<{state, msg, voltage} @ SolenoidSwitchingParams_t>", "conversionEnded @ builtin_boolean")]]
+[[rc::requires  ("[initialized \"curTime\" global_time]")]]
+[[rc::ensures("own p : {state ,msg, voltage} @ SolenoidSwitchingParams_t")]]
+[[rc::exists("changed : bool ")]]
+[[rc::ensures("{changed = if (andb (state =? 0%nat) conversionEnded) then ( if (217 <=? voltage) then (11 <=? global_time) else false) else false}")]]
+[[rc::returns("changed @ builtin_boolean")]]
+[[rc::tactics("all: try destruct state; tauto.")]]
+bool SML_isSafetyVoltageCondExists( SolenoidSwitchingParams_t* solenoidSwitchingParams_ptr, bool isConversionEnded)
+{
+	if ((solenoidSwitchingParams_ptr->state == SOLENOID_OFF) && isConversionEnded)
+    {
+        uint8_t uniqueSafetyVoltage = solenoidSwitchingParams_ptr->voltage.uniqueSafetyVoltage;
+		if ( (SAFETY_VOLTAGE_TRESHOLD == uniqueSafetyVoltage) || (uniqueSafetyVoltage > SAFETY_VOLTAGE_TRESHOLD)){
+            //curTime = Timer_getCurTime();
+			//uint8_t safetyVoltageHoldTime = getSafetyVoltageHoldTime(solenoidSwitchingParams_ptr->startTime, curTime);                         	
+			//if ( SAFETY_VOLTAGE_REQUIRED_HOLD_TIME == safetyVoltageHoldTime ||  safetyVoltageHoldTime > SAFETY_VOLTAGE_REQUIRED_HOLD_TIME){
+			if ( SAFETY_VOLTAGE_REQUIRED_HOLD_TIME == curTime ||  curTime > SAFETY_VOLTAGE_REQUIRED_HOLD_TIME){
+					return true;
+			}
+        }
+    }
+    return false;
 }
 
 /*
