_build/default/src/proofs/solswitch/generated_code.v
@@ -6,74 +6,148 @@ Set Default Proof Using "Type".
 (* Generated from [src/solswitch.c]. *)
 Section code.
   Definition file_0 : string := "src/solswitch.c".
-  Definition loc_2 : location_info := LocationInfo file_0 29 53 29 62.
-  Definition loc_3 : location_info := LocationInfo file_0 29 60 29 61.
-  Definition loc_6 : location_info := LocationInfo file_0 39 1 42 2.
-  Definition loc_7 : location_info := LocationInfo file_0 39 23 42 2.
-  Definition loc_8 : location_info := LocationInfo file_0 41 2 41 17.
-  Definition loc_9 : location_info := LocationInfo file_0 41 2 41 12.
-  Definition loc_10 : location_info := LocationInfo file_0 41 2 41 5.
-  Definition loc_11 : location_info := LocationInfo file_0 41 2 41 5.
-  Definition loc_12 : location_info := LocationInfo file_0 41 15 41 16.
-  Definition loc_13 : location_info := LocationInfo file_0 39 1 42 2.
-  Definition loc_14 : location_info := LocationInfo file_0 39 6 39 21.
-  Definition loc_15 : location_info := LocationInfo file_0 39 6 39 7.
-  Definition loc_16 : location_info := LocationInfo file_0 39 11 39 21.
-  Definition loc_17 : location_info := LocationInfo file_0 39 11 39 21.
-  Definition loc_18 : location_info := LocationInfo file_0 39 11 39 14.
-  Definition loc_19 : location_info := LocationInfo file_0 39 11 39 14.
-  Definition loc_22 : location_info := LocationInfo file_0 59 4 65 5.
-  Definition loc_23 : location_info := LocationInfo file_0 59 19 65 5.
-  Definition loc_24 : location_info := LocationInfo file_0 60 8 64 9.
-  Definition loc_25 : location_info := LocationInfo file_0 60 23 64 9.
-  Definition loc_26 : location_info := LocationInfo file_0 61 12 63 13.
-  Definition loc_27 : location_info := LocationInfo file_0 61 63 63 13.
-  Definition loc_28 : location_info := LocationInfo file_0 62 15 62 42.
-  Definition loc_29 : location_info := LocationInfo file_0 62 15 62 36.
-  Definition loc_30 : location_info := LocationInfo file_0 62 15 62 36.
-  Definition loc_31 : location_info := LocationInfo file_0 62 37 62 40.
-  Definition loc_32 : location_info := LocationInfo file_0 62 37 62 40.
-  Definition loc_33 : location_info := LocationInfo file_0 61 12 63 13.
-  Definition loc_34 : location_info := LocationInfo file_0 61 15 61 62.
-  Definition loc_35 : location_info := LocationInfo file_0 61 15 61 36.
-  Definition loc_36 : location_info := LocationInfo file_0 61 15 61 31.
-  Definition loc_37 : location_info := LocationInfo file_0 61 15 61 31.
-  Definition loc_38 : location_info := LocationInfo file_0 61 15 61 27.
-  Definition loc_39 : location_info := LocationInfo file_0 61 15 61 18.
-  Definition loc_40 : location_info := LocationInfo file_0 61 15 61 18.
-  Definition loc_41 : location_info := LocationInfo file_0 61 35 61 36.
-  Definition loc_42 : location_info := LocationInfo file_0 61 40 61 62.
-  Definition loc_43 : location_info := LocationInfo file_0 61 40 61 56.
-  Definition loc_44 : location_info := LocationInfo file_0 61 40 61 56.
-  Definition loc_45 : location_info := LocationInfo file_0 61 40 61 52.
-  Definition loc_46 : location_info := LocationInfo file_0 61 40 61 43.
-  Definition loc_47 : location_info := LocationInfo file_0 61 40 61 43.
-  Definition loc_48 : location_info := LocationInfo file_0 61 60 61 62.
-  Definition loc_49 : location_info := LocationInfo file_0 60 8 64 9.
-  Definition loc_50 : location_info := LocationInfo file_0 60 11 60 22.
-  Definition loc_51 : location_info := LocationInfo file_0 60 11 60 17.
-  Definition loc_52 : location_info := LocationInfo file_0 60 11 60 17.
-  Definition loc_53 : location_info := LocationInfo file_0 60 21 60 22.
-  Definition loc_54 : location_info := LocationInfo file_0 59 4 65 5.
-  Definition loc_55 : location_info := LocationInfo file_0 59 7 59 18.
-  Definition loc_56 : location_info := LocationInfo file_0 59 7 59 13.
-  Definition loc_57 : location_info := LocationInfo file_0 59 7 59 13.
-  Definition loc_58 : location_info := LocationInfo file_0 59 17 59 18.
-  Definition loc_61 : location_info := LocationInfo file_0 78 4 78 58.
-  Definition loc_62 : location_info := LocationInfo file_0 79 4 79 34.
-  Definition loc_63 : location_info := LocationInfo file_0 79 4 79 17.
-  Definition loc_64 : location_info := LocationInfo file_0 79 4 79 17.
-  Definition loc_65 : location_info := LocationInfo file_0 79 18 79 21.
-  Definition loc_66 : location_info := LocationInfo file_0 79 18 79 21.
-  Definition loc_67 : location_info := LocationInfo file_0 79 23 79 32.
-  Definition loc_68 : location_info := LocationInfo file_0 79 23 79 32.
-  Definition loc_69 : location_info := LocationInfo file_0 78 24 78 57.
-  Definition loc_70 : location_info := LocationInfo file_0 78 24 78 42.
-  Definition loc_71 : location_info := LocationInfo file_0 78 24 78 42.
-  Definition loc_72 : location_info := LocationInfo file_0 78 43 78 56.
-  Definition loc_73 : location_info := LocationInfo file_0 78 44 78 56.
-  Definition loc_74 : location_info := LocationInfo file_0 78 44 78 47.
-  Definition loc_75 : location_info := LocationInfo file_0 78 44 78 47.
+  Definition loc_2 : location_info := LocationInfo file_0 54 53 54 62.
+  Definition loc_3 : location_info := LocationInfo file_0 54 60 54 61.
+  Definition loc_6 : location_info := LocationInfo file_0 64 1 67 2.
+  Definition loc_7 : location_info := LocationInfo file_0 64 23 67 2.
+  Definition loc_8 : location_info := LocationInfo file_0 66 2 66 17.
+  Definition loc_9 : location_info := LocationInfo file_0 66 2 66 12.
+  Definition loc_10 : location_info := LocationInfo file_0 66 2 66 5.
+  Definition loc_11 : location_info := LocationInfo file_0 66 2 66 5.
+  Definition loc_12 : location_info := LocationInfo file_0 66 15 66 16.
+  Definition loc_13 : location_info := LocationInfo file_0 64 1 67 2.
+  Definition loc_14 : location_info := LocationInfo file_0 64 6 64 21.
+  Definition loc_15 : location_info := LocationInfo file_0 64 6 64 7.
+  Definition loc_16 : location_info := LocationInfo file_0 64 11 64 21.
+  Definition loc_17 : location_info := LocationInfo file_0 64 11 64 21.
+  Definition loc_18 : location_info := LocationInfo file_0 64 11 64 14.
+  Definition loc_19 : location_info := LocationInfo file_0 64 11 64 14.
+  Definition loc_22 : location_info := LocationInfo file_0 80 4 86 5.
+  Definition loc_23 : location_info := LocationInfo file_0 80 19 86 5.
+  Definition loc_24 : location_info := LocationInfo file_0 81 8 85 9.
+  Definition loc_25 : location_info := LocationInfo file_0 81 23 85 9.
+  Definition loc_26 : location_info := LocationInfo file_0 82 12 84 13.
+  Definition loc_27 : location_info := LocationInfo file_0 82 63 84 13.
+  Definition loc_28 : location_info := LocationInfo file_0 83 15 83 42.
+  Definition loc_29 : location_info := LocationInfo file_0 83 15 83 36.
+  Definition loc_30 : location_info := LocationInfo file_0 83 15 83 36.
+  Definition loc_31 : location_info := LocationInfo file_0 83 37 83 40.
+  Definition loc_32 : location_info := LocationInfo file_0 83 37 83 40.
+  Definition loc_33 : location_info := LocationInfo file_0 82 12 84 13.
+  Definition loc_34 : location_info := LocationInfo file_0 82 15 82 62.
+  Definition loc_35 : location_info := LocationInfo file_0 82 15 82 36.
+  Definition loc_36 : location_info := LocationInfo file_0 82 15 82 31.
+  Definition loc_37 : location_info := LocationInfo file_0 82 15 82 31.
+  Definition loc_38 : location_info := LocationInfo file_0 82 15 82 27.
+  Definition loc_39 : location_info := LocationInfo file_0 82 15 82 18.
+  Definition loc_40 : location_info := LocationInfo file_0 82 15 82 18.
+  Definition loc_41 : location_info := LocationInfo file_0 82 35 82 36.
+  Definition loc_42 : location_info := LocationInfo file_0 82 40 82 62.
+  Definition loc_43 : location_info := LocationInfo file_0 82 40 82 56.
+  Definition loc_44 : location_info := LocationInfo file_0 82 40 82 56.
+  Definition loc_45 : location_info := LocationInfo file_0 82 40 82 52.
+  Definition loc_46 : location_info := LocationInfo file_0 82 40 82 43.
+  Definition loc_47 : location_info := LocationInfo file_0 82 40 82 43.
+  Definition loc_48 : location_info := LocationInfo file_0 82 60 82 62.
+  Definition loc_49 : location_info := LocationInfo file_0 81 8 85 9.
+  Definition loc_50 : location_info := LocationInfo file_0 81 11 81 22.
+  Definition loc_51 : location_info := LocationInfo file_0 81 11 81 17.
+  Definition loc_52 : location_info := LocationInfo file_0 81 11 81 17.
+  Definition loc_53 : location_info := LocationInfo file_0 81 21 81 22.
+  Definition loc_54 : location_info := LocationInfo file_0 80 4 86 5.
+  Definition loc_55 : location_info := LocationInfo file_0 80 7 80 18.
+  Definition loc_56 : location_info := LocationInfo file_0 80 7 80 13.
+  Definition loc_57 : location_info := LocationInfo file_0 80 7 80 13.
+  Definition loc_58 : location_info := LocationInfo file_0 80 17 80 18.
+  Definition loc_61 : location_info := LocationInfo file_0 98 4 98 58.
+  Definition loc_62 : location_info := LocationInfo file_0 99 4 99 34.
+  Definition loc_63 : location_info := LocationInfo file_0 99 4 99 17.
+  Definition loc_64 : location_info := LocationInfo file_0 99 4 99 17.
+  Definition loc_65 : location_info := LocationInfo file_0 99 18 99 21.
+  Definition loc_66 : location_info := LocationInfo file_0 99 18 99 21.
+  Definition loc_67 : location_info := LocationInfo file_0 99 23 99 32.
+  Definition loc_68 : location_info := LocationInfo file_0 99 23 99 32.
+  Definition loc_69 : location_info := LocationInfo file_0 98 24 98 57.
+  Definition loc_70 : location_info := LocationInfo file_0 98 24 98 42.
+  Definition loc_71 : location_info := LocationInfo file_0 98 24 98 42.
+  Definition loc_72 : location_info := LocationInfo file_0 98 43 98 56.
+  Definition loc_73 : location_info := LocationInfo file_0 98 44 98 56.
+  Definition loc_74 : location_info := LocationInfo file_0 98 44 98 47.
+  Definition loc_75 : location_info := LocationInfo file_0 98 44 98 47.
+  Definition loc_80 : location_info := LocationInfo file_0 121 4 127 6.
+  Definition loc_81 : location_info := LocationInfo file_0 128 4 128 33.
+  Definition loc_82 : location_info := LocationInfo file_0 128 11 128 32.
+  Definition loc_83 : location_info := LocationInfo file_0 128 11 128 32.
+  Definition loc_84 : location_info := LocationInfo file_0 121 29 123 6.
+  Definition loc_85 : location_info := LocationInfo file_0 122 8 122 60.
+  Definition loc_86 : location_info := LocationInfo file_0 122 8 122 29.
+  Definition loc_87 : location_info := LocationInfo file_0 122 31 122 59.
+  Definition loc_88 : location_info := LocationInfo file_0 122 31 122 49.
+  Definition loc_89 : location_info := LocationInfo file_0 122 32 122 37.
+  Definition loc_90 : location_info := LocationInfo file_0 122 39 122 48.
+  Definition loc_91 : location_info := LocationInfo file_0 122 39 122 48.
+  Definition loc_92 : location_info := LocationInfo file_0 122 52 122 59.
+  Definition loc_93 : location_info := LocationInfo file_0 122 52 122 59.
+  Definition loc_94 : location_info := LocationInfo file_0 123 10 127 6.
+  Definition loc_95 : location_info := LocationInfo file_0 126 8 126 64.
+  Definition loc_96 : location_info := LocationInfo file_0 126 8 126 29.
+  Definition loc_97 : location_info := LocationInfo file_0 126 32 126 63.
+  Definition loc_98 : location_info := LocationInfo file_0 126 42 126 63.
+  Definition loc_99 : location_info := LocationInfo file_0 126 43 126 50.
+  Definition loc_100 : location_info := LocationInfo file_0 126 43 126 50.
+  Definition loc_101 : location_info := LocationInfo file_0 126 53 126 62.
+  Definition loc_102 : location_info := LocationInfo file_0 126 53 126 62.
+  Definition loc_103 : location_info := LocationInfo file_0 121 8 121 27.
+  Definition loc_104 : location_info := LocationInfo file_0 121 8 121 15.
+  Definition loc_105 : location_info := LocationInfo file_0 121 8 121 15.
+  Definition loc_106 : location_info := LocationInfo file_0 121 18 121 27.
+  Definition loc_107 : location_info := LocationInfo file_0 121 18 121 27.
+  Definition loc_110 : location_info := LocationInfo file_0 144 1 155 5.
+  Definition loc_111 : location_info := LocationInfo file_0 156 4 156 13.
+  Definition loc_112 : location_info := LocationInfo file_0 156 11 156 12.
+  Definition loc_113 : location_info := LocationInfo file_0 145 4 155 5.
+  Definition loc_114 : location_info := LocationInfo file_0 146 8 146 95.
+  Definition loc_115 : location_info := LocationInfo file_0 147 2 154 9.
+  Definition loc_116 : location_info := LocationInfo file_0 147 67 154 9.
+  Definition loc_117 : location_info := LocationInfo file_0 151 3 153 4.
+  Definition loc_118 : location_info := LocationInfo file_0 151 38 153 4.
+  Definition loc_119 : location_info := LocationInfo file_0 152 5 152 14.
+  Definition loc_120 : location_info := LocationInfo file_0 152 12 152 13.
+  Definition loc_121 : location_info := LocationInfo file_0 151 3 153 4.
+  Definition loc_122 : location_info := LocationInfo file_0 151 8 151 37.
+  Definition loc_123 : location_info := LocationInfo file_0 151 8 151 21.
+  Definition loc_124 : location_info := LocationInfo file_0 151 8 151 10.
+  Definition loc_125 : location_info := LocationInfo file_0 151 14 151 21.
+  Definition loc_126 : location_info := LocationInfo file_0 151 14 151 21.
+  Definition loc_127 : location_info := LocationInfo file_0 151 25 151 37.
+  Definition loc_128 : location_info := LocationInfo file_0 151 25 151 32.
+  Definition loc_129 : location_info := LocationInfo file_0 151 25 151 32.
+  Definition loc_130 : location_info := LocationInfo file_0 151 35 151 37.
+  Definition loc_131 : location_info := LocationInfo file_0 147 2 154 9.
+  Definition loc_132 : location_info := LocationInfo file_0 147 7 147 66.
+  Definition loc_133 : location_info := LocationInfo file_0 147 7 147 35.
+  Definition loc_134 : location_info := LocationInfo file_0 147 8 147 11.
+  Definition loc_135 : location_info := LocationInfo file_0 147 15 147 34.
+  Definition loc_136 : location_info := LocationInfo file_0 147 15 147 34.
+  Definition loc_137 : location_info := LocationInfo file_0 147 39 147 66.
+  Definition loc_138 : location_info := LocationInfo file_0 147 40 147 59.
+  Definition loc_139 : location_info := LocationInfo file_0 147 40 147 59.
+  Definition loc_140 : location_info := LocationInfo file_0 147 62 147 65.
+  Definition loc_141 : location_info := LocationInfo file_0 146 38 146 94.
+  Definition loc_142 : location_info := LocationInfo file_0 146 38 146 94.
+  Definition loc_143 : location_info := LocationInfo file_0 146 38 146 74.
+  Definition loc_144 : location_info := LocationInfo file_0 146 38 146 65.
+  Definition loc_145 : location_info := LocationInfo file_0 146 38 146 65.
+  Definition loc_148 : location_info := LocationInfo file_0 144 1 155 5.
+  Definition loc_149 : location_info := LocationInfo file_0 144 5 144 67.
+  Definition loc_150 : location_info := LocationInfo file_0 144 5 144 46.
+  Definition loc_151 : location_info := LocationInfo file_0 144 6 144 40.
+  Definition loc_152 : location_info := LocationInfo file_0 144 6 144 40.
+  Definition loc_153 : location_info := LocationInfo file_0 144 6 144 33.
+  Definition loc_154 : location_info := LocationInfo file_0 144 6 144 33.
+  Definition loc_155 : location_info := LocationInfo file_0 144 44 144 45.
+  Definition loc_156 : location_info := LocationInfo file_0 144 50 144 67.
+  Definition loc_157 : location_info := LocationInfo file_0 144 50 144 67.
 
   (* Definition of struct [div]. *)
   Program Definition struct_div := {|
@@ -110,12 +184,21 @@ Section code.
   |}.
   Solve Obligations with solve_struct_obligations.
 
+  (* Definition of struct [VoltageHandler_t]. *)
+  Program Definition struct_VoltageHandler_t := {|
+    sl_members := [
+      (Some "uniqueSafetyVoltage", it_layout u8)
+    ];
+  |}.
+  Solve Obligations with solve_struct_obligations.
+
   (* Definition of struct [SolenoidSwitchingParams_t]. *)
   Program Definition struct_SolenoidSwitchingParams_t := {|
     sl_members := [
       (Some "state", it_layout size_t);
       (Some "handler", layout_of struct_ComHandler_t);
-      (None, Layout 7%nat 0%nat)
+      (Some "voltage", layout_of struct_VoltageHandler_t);
+      (None, Layout 6%nat 0%nat)
     ];
   |}.
   Solve Obligations with solve_struct_obligations.
@@ -237,6 +320,113 @@ Section code.
         expr: (LocInfoE loc_62 (Call (LocInfoE loc_64 (global_SML_trySwitch)) [@{expr} LocInfoE loc_65 (use{PtrOp} (LocInfoE loc_66 ("ssp"))) ;
         LocInfoE loc_67 (use{IntOp u8} (LocInfoE loc_68 ("rxMsgSize"))) ])) ;
         Return (VOID)
+      ]> $∅
+    )%E
+  |}.
+
+  (* Definition of function [getSafetyVoltageHoldTime]. *)
+  Definition impl_getSafetyVoltageHoldTime : function := {|
+    f_args := [
+      ("startTime", it_layout u16);
+      ("curTime", it_layout u16)
+    ];
+    f_local_vars := [
+      ("safetyVoltageHoldTime", it_layout u8)
+    ];
+    f_init := "#0";
+    f_code := (
+      <[ "#0" :=
+        locinfo: loc_103 ;
+        if{IntOp i32}: LocInfoE loc_103 ((LocInfoE loc_104 (UnOp (CastOp $ IntOp i32) (IntOp u16) (LocInfoE loc_104 (use{IntOp u16} (LocInfoE loc_105 ("curTime")))))) <{IntOp i32, IntOp i32, i32} (LocInfoE loc_106 (UnOp (CastOp $ IntOp i32) (IntOp u16) (LocInfoE loc_106 (use{IntOp u16} (LocInfoE loc_107 ("startTime")))))))
+        then
+        locinfo: loc_85 ;
+          Goto "#2"
+        else
+        locinfo: loc_95 ;
+          Goto "#3"
+      ]> $
+      <[ "#1" :=
+        locinfo: loc_81 ;
+        Return (LocInfoE loc_82 (use{IntOp u8} (LocInfoE loc_83 ("safetyVoltageHoldTime"))))
+      ]> $
+      <[ "#2" :=
+        locinfo: loc_85 ;
+        LocInfoE loc_86 ("safetyVoltageHoldTime") <-{ IntOp u8 }
+          LocInfoE loc_87 (UnOp (CastOp $ IntOp u8) (IntOp i32) (LocInfoE loc_87 ((LocInfoE loc_88 ((LocInfoE loc_89 (i2v 4095 i32)) -{IntOp i32, IntOp i32} (LocInfoE loc_90 (UnOp (CastOp $ IntOp i32) (IntOp u16) (LocInfoE loc_90 (use{IntOp u16} (LocInfoE loc_91 ("startTime")))))))) +{IntOp i32, IntOp i32} (LocInfoE loc_92 (UnOp (CastOp $ IntOp i32) (IntOp u16) (LocInfoE loc_92 (use{IntOp u16} (LocInfoE loc_93 ("curTime"))))))))) ;
+        locinfo: loc_81 ;
+        Goto "#1"
+      ]> $
+      <[ "#3" :=
+        locinfo: loc_95 ;
+        LocInfoE loc_96 ("safetyVoltageHoldTime") <-{ IntOp u8 }
+          LocInfoE loc_97 (UnOp (CastOp $ IntOp u8) (IntOp i32) (LocInfoE loc_98 ((LocInfoE loc_99 (UnOp (CastOp $ IntOp i32) (IntOp u16) (LocInfoE loc_99 (use{IntOp u16} (LocInfoE loc_100 ("curTime")))))) -{IntOp i32, IntOp i32} (LocInfoE loc_101 (UnOp (CastOp $ IntOp i32) (IntOp u16) (LocInfoE loc_101 (use{IntOp u16} (LocInfoE loc_102 ("startTime"))))))))) ;
+        locinfo: loc_81 ;
+        Goto "#1"
+      ]> $∅
+    )%E
+  |}.
+
+  (* Definition of function [SML_isSafetyVoltageCondExists]. *)
+  Definition impl_SML_isSafetyVoltageCondExists (global_curTime : loc): function := {|
+    f_args := [
+      ("solenoidSwitchingParams_ptr", void*);
+      ("isConversionEnded", bool_layout)
+    ];
+    f_local_vars := [
+      ("uniqueSafetyVoltage", it_layout u8)
+    ];
+    f_init := "#0";
+    f_code := (
+      <[ "#0" :=
+        locinfo: loc_149 ;
+        if{IntOp i32}: LocInfoE loc_149 ((LocInfoE loc_150 ((LocInfoE loc_151 (use{IntOp size_t} (LocInfoE loc_152 ((LocInfoE loc_153 (!{PtrOp} (LocInfoE loc_154 ("solenoidSwitchingParams_ptr")))) at{struct_SolenoidSwitchingParams_t} "state")))) ={IntOp size_t, IntOp size_t, i32} (LocInfoE loc_155 (UnOp (CastOp $ IntOp size_t) (IntOp i32) (LocInfoE loc_155 (i2v 0 i32)))))) &&{IntOp i32, IntOp i32, i32} (LocInfoE loc_156 (UnOp (CastOp $ IntOp i32) (BoolOp) (LocInfoE loc_156 (use{BoolOp} (LocInfoE loc_157 ("isConversionEnded")))))))
+        then
+        Goto "#2"
+        else
+        locinfo: loc_111 ;
+          Goto "#7"
+      ]> $
+      <[ "#1" :=
+        locinfo: loc_111 ;
+        Return (LocInfoE loc_112 (UnOp (CastOp $ BoolOp) (IntOp i32) (LocInfoE loc_112 (i2v 0 i32))))
+      ]> $
+      <[ "#2" :=
+        "uniqueSafetyVoltage" <-{ IntOp u8 }
+          LocInfoE loc_141 (use{IntOp u8} (LocInfoE loc_142 ((LocInfoE loc_143 ((LocInfoE loc_144 (!{PtrOp} (LocInfoE loc_145 ("solenoidSwitchingParams_ptr")))) at{struct_SolenoidSwitchingParams_t} "voltage")) at{struct_VoltageHandler_t} "uniqueSafetyVoltage"))) ;
+        locinfo: loc_132 ;
+        if{IntOp i32}: LocInfoE loc_132 ((LocInfoE loc_133 ((LocInfoE loc_134 (i2v 217 i32)) ={IntOp i32, IntOp i32, i32} (LocInfoE loc_135 (UnOp (CastOp $ IntOp i32) (IntOp u8) (LocInfoE loc_135 (use{IntOp u8} (LocInfoE loc_136 ("uniqueSafetyVoltage")))))))) ||{IntOp i32, IntOp i32, i32} (LocInfoE loc_137 ((LocInfoE loc_138 (UnOp (CastOp $ IntOp i32) (IntOp u8) (LocInfoE loc_138 (use{IntOp u8} (LocInfoE loc_139 ("uniqueSafetyVoltage")))))) >{IntOp i32, IntOp i32, i32} (LocInfoE loc_140 (i2v 217 i32)))))
+        then
+        locinfo: loc_122 ;
+          Goto "#3"
+        else
+        locinfo: loc_111 ;
+          Goto "#6"
+      ]> $
+      <[ "#3" :=
+        locinfo: loc_122 ;
+        if{IntOp i32}: LocInfoE loc_122 ((LocInfoE loc_123 ((LocInfoE loc_124 (i2v 11 i32)) ={IntOp i32, IntOp i32, i32} (LocInfoE loc_125 (UnOp (CastOp $ IntOp i32) (IntOp u16) (LocInfoE loc_125 (use{IntOp u16} (LocInfoE loc_126 (global_curTime)))))))) ||{IntOp i32, IntOp i32, i32} (LocInfoE loc_127 ((LocInfoE loc_128 (UnOp (CastOp $ IntOp i32) (IntOp u16) (LocInfoE loc_128 (use{IntOp u16} (LocInfoE loc_129 (global_curTime)))))) >{IntOp i32, IntOp i32, i32} (LocInfoE loc_130 (i2v 11 i32)))))
+        then
+        locinfo: loc_119 ;
+          Goto "#4"
+        else
+        locinfo: loc_111 ;
+          Goto "#5"
+      ]> $
+      <[ "#4" :=
+        locinfo: loc_119 ;
+        Return (LocInfoE loc_120 (UnOp (CastOp $ BoolOp) (IntOp i32) (LocInfoE loc_120 (i2v 1 i32))))
+      ]> $
+      <[ "#5" :=
+        locinfo: loc_111 ;
+        Goto "#1"
+      ]> $
+      <[ "#6" :=
+        locinfo: loc_111 ;
+        Goto "#1"
+      ]> $
+      <[ "#7" :=
+        locinfo: loc_111 ;
+        Goto "#1"
       ]> $∅
     )%E
   |}.
