src/proofs/funcall/generated_code.v
@@ -5,6 +5,35 @@ Set Default Proof Using "Type".
 
 (* Generated from [src/funcall.c]. *)
 Section code.
+  Definition file_0 : string := "src/funcall.c".
+  Definition loc_2 : location_info := LocationInfo file_0 20 4 26 6.
+  Definition loc_3 : location_info := LocationInfo file_0 27 4 27 33.
+  Definition loc_4 : location_info := LocationInfo file_0 27 11 27 32.
+  Definition loc_5 : location_info := LocationInfo file_0 27 11 27 32.
+  Definition loc_6 : location_info := LocationInfo file_0 20 29 22 6.
+  Definition loc_7 : location_info := LocationInfo file_0 21 8 21 61.
+  Definition loc_8 : location_info := LocationInfo file_0 21 8 21 29.
+  Definition loc_9 : location_info := LocationInfo file_0 21 31 21 60.
+  Definition loc_10 : location_info := LocationInfo file_0 21 31 21 50.
+  Definition loc_11 : location_info := LocationInfo file_0 21 32 21 38.
+  Definition loc_12 : location_info := LocationInfo file_0 21 40 21 49.
+  Definition loc_13 : location_info := LocationInfo file_0 21 40 21 49.
+  Definition loc_14 : location_info := LocationInfo file_0 21 53 21 60.
+  Definition loc_15 : location_info := LocationInfo file_0 21 53 21 60.
+  Definition loc_16 : location_info := LocationInfo file_0 22 10 26 6.
+  Definition loc_17 : location_info := LocationInfo file_0 25 8 25 64.
+  Definition loc_18 : location_info := LocationInfo file_0 25 8 25 29.
+  Definition loc_19 : location_info := LocationInfo file_0 25 32 25 63.
+  Definition loc_20 : location_info := LocationInfo file_0 25 42 25 63.
+  Definition loc_21 : location_info := LocationInfo file_0 25 43 25 50.
+  Definition loc_22 : location_info := LocationInfo file_0 25 43 25 50.
+  Definition loc_23 : location_info := LocationInfo file_0 25 53 25 62.
+  Definition loc_24 : location_info := LocationInfo file_0 25 53 25 62.
+  Definition loc_25 : location_info := LocationInfo file_0 20 8 20 27.
+  Definition loc_26 : location_info := LocationInfo file_0 20 8 20 15.
+  Definition loc_27 : location_info := LocationInfo file_0 20 8 20 15.
+  Definition loc_28 : location_info := LocationInfo file_0 20 18 20 27.
+  Definition loc_29 : location_info := LocationInfo file_0 20 18 20 27.
 
   (* Definition of struct [div]. *)
   Program Definition struct_div := {|
@@ -33,19 +62,45 @@ Section code.
   |}.
   Solve Obligations with solve_struct_obligations.
 
-  (* Definition of struct [ComHandler]. *)
-  Program Definition struct_ComHandler := {|
-    sl_members := [
-      (Some "msg", it_layout u8)
+  (* Definition of function [getSafetyVoltageHoldTime]. *)
+  Definition impl_getSafetyVoltageHoldTime : function := {|
+    f_args := [
+      ("startTime", it_layout u16);
+      ("curTime", it_layout u16)
     ];
-  |}.
-  Solve Obligations with solve_struct_obligations.
-
-  (* Definition of struct [MyStruct]. *)
-  Program Definition struct_MyStruct := {|
-    sl_members := [
-      (Some "cmdhandler", layout_of struct_ComHandler)
+    f_local_vars := [
+      ("safetyVoltageHoldTime", it_layout u8)
     ];
+    f_init := "#0";
+    f_code := (
+      <[ "#0" :=
+        locinfo: loc_25 ;
+        if{IntOp i32}: LocInfoE loc_25 ((LocInfoE loc_26 (UnOp (CastOp $ IntOp i32) (IntOp u16) (LocInfoE loc_26 (use{IntOp u16} (LocInfoE loc_27 ("curTime")))))) <{IntOp i32, IntOp i32, i32} (LocInfoE loc_28 (UnOp (CastOp $ IntOp i32) (IntOp u16) (LocInfoE loc_28 (use{IntOp u16} (LocInfoE loc_29 ("startTime")))))))
+        then
+        locinfo: loc_7 ;
+          Goto "#2"
+        else
+        locinfo: loc_17 ;
+          Goto "#3"
+      ]> $
+      <[ "#1" :=
+        locinfo: loc_3 ;
+        Return (LocInfoE loc_4 (use{IntOp u8} (LocInfoE loc_5 ("safetyVoltageHoldTime"))))
+      ]> $
+      <[ "#2" :=
+        locinfo: loc_7 ;
+        LocInfoE loc_8 ("safetyVoltageHoldTime") <-{ IntOp u8 }
+          LocInfoE loc_9 (UnOp (CastOp $ IntOp u8) (IntOp i32) (LocInfoE loc_9 ((LocInfoE loc_10 ((LocInfoE loc_11 (i2v 65535 i32)) -{IntOp i32, IntOp i32} (LocInfoE loc_12 (UnOp (CastOp $ IntOp i32) (IntOp u16) (LocInfoE loc_12 (use{IntOp u16} (LocInfoE loc_13 ("startTime")))))))) +{IntOp i32, IntOp i32} (LocInfoE loc_14 (UnOp (CastOp $ IntOp i32) (IntOp u16) (LocInfoE loc_14 (use{IntOp u16} (LocInfoE loc_15 ("curTime"))))))))) ;
+        locinfo: loc_3 ;
+        Goto "#1"
+      ]> $
+      <[ "#3" :=
+        locinfo: loc_17 ;
+        LocInfoE loc_18 ("safetyVoltageHoldTime") <-{ IntOp u8 }
+          LocInfoE loc_19 (UnOp (CastOp $ IntOp u8) (IntOp i32) (LocInfoE loc_20 ((LocInfoE loc_21 (UnOp (CastOp $ IntOp i32) (IntOp u16) (LocInfoE loc_21 (use{IntOp u16} (LocInfoE loc_22 ("curTime")))))) -{IntOp i32, IntOp i32} (LocInfoE loc_23 (UnOp (CastOp $ IntOp i32) (IntOp u16) (LocInfoE loc_23 (use{IntOp u16} (LocInfoE loc_24 ("startTime"))))))))) ;
+        locinfo: loc_3 ;
+        Goto "#1"
+      ]> $∅
+    )%E
   |}.
-  Solve Obligations with solve_struct_obligations.
 End code.
