src/proofs/solswitch/generated_spec.v
@@ -46,13 +46,55 @@ Section spec.
     SimplifyGoalVal v_ (patt__ @ ComHandler_t)%I (Some 100%N) :=
     λ T, i2p (simplify_goal_val_eq v_ _ _ T (ComHandler_t_unfold _)).
 
+  (* Definition of type [VoltageHandler_t]. *)
+  Definition VoltageHandler_t_rec : (nat -d> typeO) → (nat -d> typeO) := (λ self unique_voltage,
+    struct struct_VoltageHandler_t [@{type}
+      (unique_voltage @ (int (u8)))
+    ]
+  )%I.
+  Typeclasses Opaque VoltageHandler_t_rec.
+
+  Global Instance VoltageHandler_t_rec_ne : Contractive VoltageHandler_t_rec.
+  Proof. solve_type_proper. Qed.
+  Global Instance VoltageHandler_t_rec_proper : Proper ((≡) ==> (≡)) VoltageHandler_t_rec.
+  Proof. apply contractive_proper, _. Qed.
+
+  Definition VoltageHandler_t : rtype := {|
+    rty_type := nat;
+    rty r__ := VoltageHandler_t_rec (fixp VoltageHandler_t_rec) r__
+  |}.
+
+  Lemma VoltageHandler_t_unfold (unique_voltage : nat):
+    (unique_voltage @ VoltageHandler_t)%I ≡@{type} (
+      struct struct_VoltageHandler_t [@{type}
+        (unique_voltage @ (int (u8)))
+      ]
+    )%I.
+  Proof. apply: (fixp_unfold' VoltageHandler_t_rec). Qed.
+
+  Global Instance VoltageHandler_t_simplify_hyp_place_inst_generated l_ β_ patt__:
+    SimplifyHypPlace l_ β_ (patt__ @ VoltageHandler_t)%I (Some 100%N) :=
+    λ T, i2p (simplify_hyp_place_eq l_ β_ _ _ T (VoltageHandler_t_unfold _)).
+  Global Instance VoltageHandler_t_simplify_goal_place_inst_generated l_ β_ patt__:
+    SimplifyGoalPlace l_ β_ (patt__ @ VoltageHandler_t)%I (Some 100%N) :=
+    λ T, i2p (simplify_goal_place_eq l_ β_ _ _ T (VoltageHandler_t_unfold _)).
+
+  Global Instance VoltageHandler_t_simplify_hyp_val_inst_generated v_ patt__:
+    SimplifyHypVal v_ (patt__ @ VoltageHandler_t)%I (Some 100%N) :=
+    λ T, i2p (simplify_hyp_val_eq v_ _ _ T (VoltageHandler_t_unfold _)).
+  Global Instance VoltageHandler_t_simplify_goal_val_inst_generated v_ patt__:
+    SimplifyGoalVal v_ (patt__ @ VoltageHandler_t)%I (Some 100%N) :=
+    λ T, i2p (simplify_goal_val_eq v_ _ _ T (VoltageHandler_t_unfold _)).
+
   (* Definition of type [SolenoidSwitchingParams_t]. *)
-  Definition SolenoidSwitchingParams_t_rec : (nat * nat -d> typeO) → (nat * nat -d> typeO) := (λ self patt__,
-    let state := patt__.1 in
-    let msg := patt__.2 in
+  Definition SolenoidSwitchingParams_t_rec : (nat * nat * nat -d> typeO) → (nat * nat * nat -d> typeO) := (λ self patt__,
+    let state := patt__.1.1 in
+    let msg := patt__.1.2 in
+    let voltage := patt__.2 in
     struct struct_SolenoidSwitchingParams_t [@{type}
       (state @ (int (size_t))) ;
-      ((msg @ (ComHandler_t)))
+      ((msg @ (ComHandler_t))) ;
+      ((voltage @ (VoltageHandler_t)))
     ]
   )%I.
   Typeclasses Opaque SolenoidSwitchingParams_t_rec.
@@ -63,17 +105,19 @@ Section spec.
   Proof. apply contractive_proper, _. Qed.
 
   Definition SolenoidSwitchingParams_t : rtype := {|
-    rty_type := nat * nat;
+    rty_type := nat * nat * nat;
     rty r__ := SolenoidSwitchingParams_t_rec (fixp SolenoidSwitchingParams_t_rec) r__
   |}.
 
-  Lemma SolenoidSwitchingParams_t_unfold (patt__ : nat * nat):
+  Lemma SolenoidSwitchingParams_t_unfold (patt__ : nat * nat * nat):
     (patt__ @ SolenoidSwitchingParams_t)%I ≡@{type} (
-      let state := patt__.1 in
-      let msg := patt__.2 in
+      let state := patt__.1.1 in
+      let msg := patt__.1.2 in
+      let voltage := patt__.2 in
       struct struct_SolenoidSwitchingParams_t [@{type}
         (state @ (int (size_t))) ;
-        ((msg @ (ComHandler_t)))
+        ((msg @ (ComHandler_t))) ;
+        ((voltage @ (VoltageHandler_t)))
       ]
     )%I.
   Proof. apply: (fixp_unfold' SolenoidSwitchingParams_t_rec). Qed.
@@ -179,19 +223,34 @@ Section spec.
 
   (* Specifications for function [SML_switchTheSolenoid]. *)
   Definition type_of_SML_switchTheSolenoid :=
-    fn(∀ (state, msg, p) : nat * nat * loc; (p @ (&own ((state, msg) @ (SolenoidSwitchingParams_t)))); True)
-      → ∃ new_state : nat, (void); (p ◁ₗ (( new_state ,msg) @ (SolenoidSwitchingParams_t))) ∗ ⌜new_state = (if Nat.eqb state 0%nat then 1%nat else state)⌝.
+    fn(∀ (state, msg, p, voltage) : nat * nat * loc * nat; (p @ (&own ((state, msg, voltage) @ (SolenoidSwitchingParams_t)))); True)
+      → ∃ new_state : nat, (void); (p ◁ₗ ((new_state ,msg, voltage) @ (SolenoidSwitchingParams_t))) ∗ ⌜new_state = (if Nat.eqb state 0%nat then 1%nat else state)⌝.
 
   (* Specifications for function [SML_trySwitch]. *)
   Definition type_of_SML_trySwitch :=
-    fn(∀ (state, msg, len, p) : nat * nat * nat * loc; (p @ (&own ((state, msg) @ (SolenoidSwitchingParams_t)))), (len @ (int (u8))); True)
-      → ∃ (new_msg, new_state) : nat * nat, (void); (p ◁ₗ (( new_state ,new_msg) @ (SolenoidSwitchingParams_t))) ∗ ⌜((new_msg = 7%nat ∨ new_msg = 12%nat) ∧ (len = 8%nat) ∧ (state = 0%nat) -> (new_state = 1%nat)) ∨ (new_state = state)⌝.
+    fn(∀ (state, msg, len, p, voltage) : nat * nat * nat * loc * nat; (p @ (&own ((state, msg, voltage) @ (SolenoidSwitchingParams_t)))), (len @ (int (u8))); True)
+      → ∃ (new_msg, new_state) : nat * nat, (void); (p ◁ₗ (( new_state ,new_msg, voltage) @ (SolenoidSwitchingParams_t))) ∗ ⌜((new_msg = 7%nat ∨ new_msg = 12%nat) ∧ (len = 8%nat) ∧ (state = 0%nat) -> (new_state = 1%nat)) ∨ (new_state = state)⌝.
 
   (* Specifications for function [SML_handleReceivedMsgs]. *)
   Definition type_of_SML_handleReceivedMsgs :=
-    fn(∀ (state, msg, p) : nat * nat * loc; (p @ (&own ((state, msg) @ (SolenoidSwitchingParams_t)))); True)
-      → ∃ (new_msg, new_state) : nat * nat, (void); (p ◁ₗ (( new_state ,new_msg) @ (SolenoidSwitchingParams_t))) ∗ ⌜((new_msg = 7%nat ∨ new_msg = 12%nat) ∧  (state = 0%nat) -> (new_state = 1%nat)) ∨ (new_state = state)⌝.
+    fn(∀ (state, msg, p, voltage) : nat * nat * loc * nat; (p @ (&own ((state, msg, voltage) @ (SolenoidSwitchingParams_t)))); True)
+      → ∃ (new_msg, new_state) : nat * nat, (void); (p ◁ₗ ((new_state ,new_msg, voltage) @ (SolenoidSwitchingParams_t))).
+
+  (* Specifications for function [Timer_getCurTime]. *)
+  Definition type_of_Timer_getCurTime :=
+    fn(∀ time : nat; True) → ∃ () : (), (time @ (int (u16))); True.
+
+  (* Specifications for function [getSafetyVoltageHoldTime]. *)
+  Definition type_of_getSafetyVoltageHoldTime :=
+    fn(∀ (last_time, current_time) : nat * nat; (last_time @ (int (u16))), (current_time @ (int (u16))); True)
+      → ∃ () : (), ((last_time > current_time ? (65535 - last_time + current_time) : (current_time - last_time)) @ (int (u8))); True.
+
+  (* Specifications for function [SML_isSafetyVoltageCondExists]. *)
+  Definition type_of_SML_isSafetyVoltageCondExists :=
+    fn(∀ (state, msg, conversionEnded, voltage, p, global_time) : nat * nat * bool * nat * loc * nat; (p @ (&own ((state, msg, voltage) @ (SolenoidSwitchingParams_t)))), (conversionEnded @ (builtin_boolean)); (initialized "curTime" global_time))
+      → ∃ changed : bool, (changed @ (builtin_boolean)); (p ◁ₗ ((state ,msg, voltage) @ (SolenoidSwitchingParams_t))) ∗ ⌜changed = if (andb (state =? 0%nat) conversionEnded) then ( if (217 <=? voltage) then (11 <=? global_time) else false) else false⌝.
 End spec.
 
 Typeclasses Opaque ComHandler_t_rec.
+Typeclasses Opaque VoltageHandler_t_rec.
 Typeclasses Opaque SolenoidSwitchingParams_t_rec.
