src/proofs/funcall/generated_proof_getSafetyVoltageHoldTime.v
@@ -1,0 +1,28 @@
+From refinedc.typing Require Import typing.
+From refinedc.project.learning.src.funcall Require Import generated_code.
+From refinedc.project.learning.src.funcall Require Import generated_spec.
+Set Default Proof Using "Type".
+
+(* Generated from [src/funcall.c]. *)
+Section proof_getSafetyVoltageHoldTime.
+  Context `{!typeG Σ} `{!globalG Σ}.
+
+  (* Typing proof for [getSafetyVoltageHoldTime]. *)
+  Lemma type_getSafetyVoltageHoldTime :
+    ⊢ typed_function impl_getSafetyVoltageHoldTime type_of_getSafetyVoltageHoldTime.
+  Proof.
+    Open Scope printing_sugar.
+    start_function "getSafetyVoltageHoldTime" ([last_time current_time]) => arg_startTime arg_curTime local_safetyVoltageHoldTime.
+    prepare_parameters (last_time current_time).
+    split_blocks ((
+      ∅
+    )%I : gmap label (iProp Σ)) ((
+      ∅
+    )%I : gmap label (iProp Σ)).
+    - repeat liRStep; liShow.
+      all: print_typesystem_goal "getSafetyVoltageHoldTime" "#0".
+    Unshelve. all: li_unshelve_sidecond; sidecond_hook; prepare_sideconditions; normalize_and_simpl_goal; try solve_goal; unsolved_sidecond_hook.
+    all: print_sidecondition_goal "getSafetyVoltageHoldTime".
+    Unshelve. all: try done; try apply: inhabitant; print_remaining_shelved_goal "getSafetyVoltageHoldTime".
+  Qed.
+End proof_getSafetyVoltageHoldTime.
